Parametrize over Curve vale precondition, following @protz advice

code/hpke/Hacl.HPKE.Curve64_CP128_SHA512.fst
@@ -11,10 +11,10 @@ friend Hacl.Meta.HPKE
 
 #set-options "--fuel 0 --ifuel 0"
 
-let setupBaseI = hpke_setupBaseI_higher #cs True IHK.hkdf_expand512 IHK.hkdf_extract512 IHash.hash_sha512 IDH.secret_to_public_c64 IDH.dh_c64
+let setupBaseI = hpke_setupBaseI_higher #cs vale_p IHK.hkdf_expand512 IHK.hkdf_extract512 IHash.hash_sha512 IDH.secret_to_public_c64 IDH.dh_c64
 
-let setupBaseR = hpke_setupBaseR_higher #cs True IHK.hkdf_expand512 IHK.hkdf_extract512 IHash.hash_sha512 IDH.dh_c64 IDH.secret_to_public_c64
+let setupBaseR = hpke_setupBaseR_higher #cs vale_p IHK.hkdf_expand512 IHK.hkdf_extract512 IHash.hash_sha512 IDH.dh_c64 IDH.secret_to_public_c64
 
-let sealBase = hpke_sealBase_higher #cs True setupBaseI IAEAD.aead_encrypt_cp128
+let sealBase = hpke_sealBase_higher #cs vale_p setupBaseI IAEAD.aead_encrypt_cp128
 
-let openBase = hpke_openBase_higher #cs True setupBaseR IAEAD.aead_decrypt_cp128
+let openBase = hpke_openBase_higher #cs vale_p setupBaseR IAEAD.aead_decrypt_cp128
